finish characterization of fo terms

src/fol/syntax.lean
@@ -60,7 +60,20 @@ section
 end
 
 def is_arity (num_sorts : nat) (t : type) : bool := 
-if t.infer_arity_kind num_sorts = arity.kind.none then ff else tt 
+if t.infer_arity_kind num_sorts = arity.kind.none then ff else tt
+
+theorem is_arity_iff (num_sorts : nat) (t : type) :
+  is_arity num_sorts t = tt ↔ 
+    ((∀ t' ∈ get_arg_types t, is_sort num_sorts t' = tt) ∧
+      (is_sort num_sorts (get_return_type t) = tt ∨ 
+      (is_prop (get_return_type t) = tt))) :=
+begin
+  induction t with _ _ t₁ t₂ ih₁ ih₂; 
+    simp [is_arity, infer_arity_kind, is_sort, is_prop] at *,
+  { cases t; simp [is_sort, is_prop], by_cases h : t < num_sorts; simp [h] },
+  by_cases h : is_sort num_sorts t₁ = tt; simp [h] at *,
+  exact ih₂ 
+end
 
 /--
 If `t` is an arity, `infer_arity num_sorts t` returns `some (alist, r)` where `alist` is the list of argument types, and `r` is the return type.
@@ -142,6 +155,10 @@ end type
 
 namespace term
 
+-- a hack for handling of quantifiers: fix later
+def inhabited_type : inhabited type := ⟨mk_nat⟩ 
+local attribute [instance] inhabited_type
+
 namespace const
 
 def in_fo_language (L : fol.language) : const → bool
@@ -158,14 +175,18 @@ def in_fo_language (L : fol.language) : const → bool
   | (term.const.kind.or)      := if t = (mk_prop ⇒ mk_prop ⇒ mk_prop) then l.empty else bool.ff
   | (term.const.kind.implies) := if t = (mk_prop ⇒ mk_prop ⇒ mk_prop) then l.empty else bool.ff
   | (term.const.kind.iff)     := if t = (mk_prop ⇒ mk_prop ⇒ mk_prop) then l.empty else bool.ff
-  | (term.const.kind.all)     := match l with 
-                                 | [t'] := if t = (t' ⇒ t' ⇒ t') then bool.tt else bool.ff
+  | (term.const.kind.all)     := let t' := l.head in 
+                                 if t = (t' ⇒ mk_prop ⇒ mk_prop) then bool.tt else bool.ff
+                                  /- match l with 
+                                 | [t'] := if t = (t' ⇒ mk_prop ⇒ mk_prop) then bool.tt else bool.ff
                                  | _     := bool.ff
-                                 end
-  | (term.const.kind.ex)      := match l with 
-                                 | [t'] := if t = (t' ⇒ t' ⇒ t') then bool.tt else bool.ff
+                                 end -/
+  | (term.const.kind.ex)      := let t' := l.head in 
+                                 if t = (t' ⇒ mk_prop ⇒ mk_prop) then bool.tt else bool.ff
+                                 /- match l with 
+                                 | [t'] := if t = (t' ⇒ mk_prop ⇒ mk_prop) then bool.tt else bool.ff
                                  | _     := bool.ff
-                                 end
+                                 end -/
   | _                         := bool.ff
   end
 
@@ -176,10 +197,27 @@ def in_fo_language (L : fol.language) (σ : list type): term → bool
 | (term.Var n)      := if h : n < σ.length then (σ.nth_le n h).is_fo_sort L else bool.ff  
 | (term.Const c)    := c.in_fo_language L = tt
 | (term.App t₁ t₂)  := in_fo_language t₁ && in_fo_language t₂ = tt
-| (term.Abs s ty t) := in_fo_language t = ff
+| (term.Abs s ty t) := ff
 
-def is_fo_term (L : fol.language) (t : term) (σ : list type) : Prop :=
-t.is_well_typed σ ∧ in_fo_language L σ t = tt ∧ (t.typeof σ).is_fo_sort L = tt
+theorem is_sort_of_is_var {L : fol.language} {t : term} {σ : list type} : 
+  t.is_var = tt → in_fo_language L σ t = tt → 
+    (t.typeof σ).is_fo_sort L = tt :=
+by { cases t with n; simp, by_cases h : n < σ.length; simp [h, typeof] }
+
+theorem is_arity_of_is_const {L : fol.language} {t : term} {σ : list type} :
+  t.is_const = tt → in_fo_language L σ t = tt → 
+      (t.typeof σ).get_return_type.is_sort L.num_sorts = tt → 
+    (t.typeof σ).is_arity L.num_sorts = tt :=
+begin
+  have h₀ : type.is_sort (L.num_sorts) (type.get_return_type mk_prop) = ff,
+    reflexivity,
+  induction t with _ c; simp,
+  cases c; cases c_symb; simp [const.in_fo_language, const.in_fo_language._match_1, typeof],
+  { by_cases h : c_symb < L.num_symbols; simp [h],
+    intro heq, rw [← heq, L.arities_ok], simp }, 
+  all_goals {
+    try { intro heq; simp [heq, type.is_arity, type.get_return_type, h₀] } }
+end
 
 theorem in_fo_language_mk_app (L : fol.language) (t : term) (l : list term) (σ : list type) :
   (mk_app t l).in_fo_language L σ = tt ↔ 
@@ -189,23 +227,103 @@ begin
   intro t, rw ih, simp, rw [← and.assoc, @and.comm (_ = tt)],
 end
 
+theorem in_fo_language_get_app_fn {L : fol.language} {t : term} {σ : list type} : 
+  t.in_fo_language L σ = tt → (get_app_fn t).in_fo_language L σ = tt:=
+begin
+  induction t with _ _ _ _ ih; simp,
+  intros h h', rw ih h,
+end
+
+theorem in_fo_language_cases {L : fol.language} {t : term} {σ : list type} : 
+  t.in_fo_language L σ = tt → t.is_const = tt ∨ t.is_var = tt ∨ t.is_app = tt :=
+by { cases t; simp }
+
+theorem is_const_get_app_fn_of_in_fo_language {L : fol.language} {t : term} {σ : list type} 
+    (h : in_fo_language L σ t = tt) :
+  t.is_well_typed σ → t.is_app = tt → t.get_app_fn.is_const = tt :=
+begin
+  intros h₀ h₁,
+  have := in_fo_language_cases (in_fo_language_get_app_fn h),
+  cases this,
+  { revert this, cases t; simp },
+  cases this; revert this,
+  { intro h', 
+    have h₂ := is_arrow_get_app_fn_of_is_app h₀ h₁,
+    have h₃ := is_sort_of_is_var h' (in_fo_language_get_app_fn h),
+    revert h₂ h₃,
+    generalize : t.get_app_fn.typeof σ = T,
+    cases T; simp [type.is_fo_sort, type.is_sort] },
+  intro h',
+  rw not_is_app_get_app_fn at h', contradiction
+end
+
+def is_fo_term (L : fol.language) (t : term) (σ : list type) : Prop :=
+t.is_well_typed σ ∧ in_fo_language L σ t = tt ∧ (t.typeof σ).is_fo_sort L = tt
+
 private theorem hoist_precondition {A B C : Prop} (h₀ : A → C) (h₁ : B → C) (h : C → (A ↔ B)) :
   A ↔ B :=
 iff.intro (λ hA, (h (h₀ hA)).mp hA) (λ hB, (h (h₁ hB)).mpr hB)
-
-/-
-both sides imply: is not an arrow, is well_typed, ...
--/
 
 theorem is_fo_term_iff_aux (L : fol.language) (t : term) (σ : list type) (h : t.is_app = tt):
   is_fo_term L t σ ↔ 
     let fn := t.get_app_fn,
           args := t.get_app_args,
           fn_type := fn.typeof σ in
-        fn.is_const = tt ∧ fn.in_fo_language L σ = tt ∧ fn_type.get_return_type.is_fo_sort L = tt ∧ 
-        (∀ t' ∈ args, is_fo_term L t σ) ∧
+        fn.in_fo_language L σ = tt ∧ 
+        fn.is_const = tt ∧ 
+        fn_type.get_return_type.is_fo_sort L = tt ∧ 
+        (∀ t' ∈ args, is_fo_term L t' σ) ∧
         fn_type.get_arg_types = t.get_app_args.map (λ t', t'.typeof σ) :=
-sorry  
+begin
+  have : is_fo_term L t σ →  t.is_well_typed σ,
+  { unfold is_fo_term, rintros ⟨h₁, h₂, h₃⟩, exact h₁},
+  apply hoist_precondition this,
+  { rintros ⟨h₁, h₂, h₃, h₄, h₅⟩, 
+    rw is_well_typed_iff',
+    split, { apply is_well_typed_of_is_const h₂ },
+    split, { intros t' ht', exact (h₄ _ ht').left },
+    rw h₅ },
+  intro is_well_typed_t,
+  have : is_fo_term L t σ → (t.typeof σ).is_arrow = ff,
+  { rintros ⟨h₁, h₂, h₃⟩, rw [type.is_not_arrow_of_is_sort h₃] },
+  apply hoist_precondition this,
+  { rintros ⟨h₁, h₂, h₃, h₄, h₅⟩, 
+    apply (type_is_not_arrow_iff is_well_typed_t).mpr, 
+    right, right, exact ⟨h, h₅⟩ },
+  intro is_not_arrow_t,
+  have in_fo_language_iff : in_fo_language L σ t = tt ↔ 
+    in_fo_language L σ t.get_app_fn = tt ∧ 
+      ∀ t' ∈ t.get_app_args, in_fo_language L σ t' = tt,
+  { transitivity, { rw [← mk_app_get_app t, in_fo_language_mk_app] },
+    apply iff.refl },
+  have : is_fo_term L t σ → in_fo_language L σ t = tt, 
+  { unfold is_fo_term, rintros ⟨h₁, h₂, h₃⟩, exact h₂ },
+  apply hoist_precondition this,
+  { rintros ⟨h₁, h₂, h₃, h₄, h₅⟩, apply in_fo_language_iff.mpr,
+    split, apply h₁, intros t' ht', apply (h₄ t' ht').right.left  },
+  intro in_fo_language_t,
+  have h' := is_const_get_app_fn_of_in_fo_language in_fo_language_t is_well_typed_t h,
+  have h'' := (type_is_not_arrow' is_well_typed_t).mp is_not_arrow_t,
+  have h''' := is_well_typed_iff'.mp is_well_typed_t, 
+  unfold is_fo_term,
+  simp [is_well_typed_t, is_not_arrow_t, in_fo_language_t, 
+    in_fo_language_iff.mp in_fo_language_t, h', h''  ],  
+  rw ← typeof_eq_of_not_is_arrow is_not_arrow_t is_well_typed_t,
+  split,
+  { intro h'''', split, exact h'''', 
+    intros t' ht',
+    split, exact h'''.right.left t' ht',
+    split, apply (in_fo_language_iff.mp in_fo_language_t).right t' ht',
+    have h₅ : t'.typeof σ ∈ type.get_arg_types (typeof (get_app_fn t) σ),
+    { rw h'', apply list.mem_map_of_mem _ ht' },
+    have : type.is_arity L.num_sorts (typeof (get_app_fn t) σ) = tt, 
+    { apply is_arity_of_is_const h' (in_fo_language_iff.mp in_fo_language_t).left,
+      rw ← typeof_eq_of_not_is_arrow is_not_arrow_t is_well_typed_t,
+      exact h'''' },
+    have := ((type.is_arity_iff _ _).mp this).left _ h₅,  
+    exact this },
+  exact and.left
+end
 
 theorem is_fo_term_iff (L : fol.language) (t : term) (σ : list type) :
   is_fo_term L t σ ↔ 
@@ -215,8 +333,9 @@ theorem is_fo_term_iff (L : fol.language) (t : term) (σ : list type) :
       let fn := t.get_app_fn,
           args := t.get_app_args,
           fn_type := fn.typeof σ in
-        fn.is_const = tt ∧ fn.in_fo_language L σ = tt ∧ fn_type.get_return_type.is_fo_sort L = tt ∧ 
-        (∀ t' ∈ args, is_fo_term L t σ) ∧
+         fn.in_fo_language L σ = tt ∧ 
+         fn.is_const = tt ∧ fn_type.get_return_type.is_fo_sort L = tt ∧ 
+        (∀ t' ∈ args, is_fo_term L t' σ) ∧
         fn_type.get_arg_types = t.get_app_args.map (λ t', t'.typeof σ)) :=
 begin
   induction t,
